8: python impl and isValid

Matei.dfy
@@ -34,6 +34,11 @@ function edges_in_graph(g: Graph): set<Edge>
   case Graph(v, e) => e
 }
 
+predicate isValid(graph: Graph)
+{
+  forall e :: e in graph.edges ==> e.source in graph.nodes && e.destination in graph.nodes
+}
+
 method Main(){
   var node1 := V(1);
   var node2 := V(2);
@@ -43,5 +48,28 @@ method Main(){
   var edge2 := Edge(node2,node3, W(4));
 
   var graph1 := Graph({node1,node2,node3}, {edge1,edge2});
+}
+
+predicate EmptySet<T(==)>() { {} is set<T> }
+
+method check_if_set_empty(s: set<int>) returns (IsEmpty:bool)
+{
+  IsEmpty := s == {};
+}
+
+method hasNegativeCycle(graph: Graph) returns (hasNegative: bool)
+{
+  var nodess := graph.nodes;
+  var edgess := graph.edges;
+
+  if nodess == {} {
+    hasNegative := false;
+    return;
+  }
+  else{
+    hasNegative := true;
+    return;
+  }
+
 }
 
